examples/primitives/bignum.fst
@@ -5,8 +5,8 @@ open FStar.Ghost
 open Axioms
 open IntLib
 open IntLibLemmas
-open Sint
-open FStar.UInt63
+open SInt
+open SInt.UInt63
 open SBuffer
 open Bigint
 open Parameters
@@ -42,18 +42,18 @@ val finalize: b:bigint -> ST unit
 
 let finalize b =
   admit();
-  let mask_26 = (FStar.UInt63.one ^<< 26) ^- FStar.UInt63.one in
-  let mask2_26m5 = mask_26 ^- (FStar.UInt63.one ^<< 2) in
+  let mask_26 = (SInt.UInt63.one ^<< 26) ^- SInt.UInt63.one in
+  let mask2_26m5 = mask_26 ^- (SInt.UInt63.one ^<< 2) in
   let b0 = index b 0 in
   let b1 = index b 1 in
   let b2 = index b 2 in
   let b3 = index b 3 in
   let b4 = index b 4 in
-  let mask = FStar.UInt63.eq b4 mask_26 in
-  let mask = FStar.UInt63.eq b3 mask_26 ^& mask in 
-  let mask = FStar.UInt63.eq b2 mask_26 ^& mask in 
-  let mask = FStar.UInt63.eq b1 mask_26 ^& mask in 
-  let mask = FStar.UInt63.gte b0 mask2_26m5 ^& mask in 
+  let mask = SInt.UInt63.eq b4 mask_26 in
+  let mask = SInt.UInt63.eq b3 mask_26 ^& mask in 
+  let mask = SInt.UInt63.eq b2 mask_26 ^& mask in 
+  let mask = SInt.UInt63.eq b1 mask_26 ^& mask in 
+  let mask = SInt.UInt63.gte b0 mask2_26m5 ^& mask in 
   upd b 0 (b0 ^- (mask ^& mask2_26m5));
   upd b 1 (b1 ^- (b1 ^& mask));
   upd b 2 (b2 ^- (b2 ^& mask));
@@ -135,6 +135,8 @@ val fsum': a:bigint -> b:bigint{disjoint a b} -> ST unit
 val gcut: f:(unit -> GTot Type) -> Pure unit (requires (f ())) (ensures f)
 let gcut f = ()
 
+assume val gassume: f:(unit -> GTot Type) -> Pure unit (requires (True)) (ensures f)
+
 let fsum' a b =
   gcut (fun _ -> pow2 26 + pow2 26 <= pow2 27);
   IntLibLemmas.pow2_increases 63 27;
@@ -156,7 +158,6 @@ let fsum' a b =
     (requires (forall (i:nat). {:pattern (v (get h1 b i))} i < len ==> v (get h0 a i) * v s = v (get h1 b i)))
     (ensures (eval h0 a len * v s = eval h1 b len)) 
 let rec gscalar_multiplication_lemma h0 h1 a b s len =
-//  admit();
   match len with
   | 0 -> () 
   | _ -> 
@@ -185,8 +186,6 @@ let scalarProduct (h0:heap) (h1:heap) (ctr:nat) (a:bigint) (s:uint63) (res:bigin
   live h0 a /\ live h1 res /\ ctr <= norm_length
   /\ (forall (i:nat). {:pattern (v (get h1 res i))} i < ctr ==> v (get h1 res i) = v (get h0 a i) * v s)
 
-#set-options "--lax"
-
 val scalar_multiplication_aux: res:bigint -> a:bigint{disjoint res a} -> s:uint63 -> ctr:nat -> ST unit
   (requires (fun h -> live h res /\ live h a /\ ctr <= norm_length
     /\ (forall (i:nat). {:pattern (v (get h a i))} i < ctr ==> v (get h a i) * v s < pow2 63) ))
@@ -198,25 +197,26 @@ let rec scalar_multiplication_aux res a s ctr =
   | 0 -> ()
   | _ -> let i = ctr - 1 in 
          let ai = index a i in
-//	 cut (True /\ v (get h0 a i) * v s < pow2 63);
+	 gcut (fun _ -> v (get h0 a i) * v s < pow2 63);
 	 let resi = ai ^* s in
 	 upd res i resi; 
 	 let h1 = ST.get() in
 	 eq_lemma h0 h1 a (only res);
 	 scalar_multiplication_aux res a s i; 
 	 let h2 = ST.get() in
-//	 cut (modifies_buf (only res) h0 h1); cut (equal h0 a h2 a); 	 
-//	 cut (forall (i:nat). {:pattern (v (get h2 res (ctr+i-1)))} i < length res - ctr + 1 ==> v (get h2 res (ctr-1 + i)) = v (get h1 res (ctr-1+i)));  
-//	 cut (forall (i:nat). {:pattern (v (get h2 res (ctr+(i-1))))} i < length res - ctr + 1 ==> v (get h2 res (ctr+i-1)) = v (get h1 res (ctr+i-1)));  
+	 gcut (fun _ -> modifies_buf (only res) h0 h1); 
+	 gcut (fun _ -> equal h0 a h2 a); 	 
+	 cut (forall (i:nat). {:pattern (v (get h2 res (ctr+i-1)))} i < length res - ctr + 1 ==> v (get h2 res (ctr-1 + i)) = v (get h1 res (ctr-1+i)));  
+	 cut (forall (i:nat). {:pattern (v (get h2 res (ctr+(i-1))))} i < length res - ctr + 1 ==> v (get h2 res (ctr+i-1)) = v (get h1 res (ctr+i-1)));  
 	 cut (forall (i:nat). {:pattern (get h2 res (ctr+i))} i < length res - ctr ==> v (get h2 res (ctr-1+(i+1))) = v (get h1 res (ctr-1+i+1)));  
-//	 cut (equalSub h1 res ctr h2 res ctr (length res - ctr)); 
+	 gcut (fun _ -> equalSub h1 res ctr h2 res ctr (length res - ctr)); 
 	 cut (forall (i:nat). {:pattern (v (get h2 res i))} i < ctr - 1 ==> v (get h2 res i) = v (get h1 a i) * v s); 
 	 cut (forall (i:nat). {:pattern (v (get h1 res i))} (i < length res /\ i <> ctr-1) ==> v (get h1 res i) = v (get h0 res i)); 
-//	 cut (True /\ v (get h2 res (ctr-1+0)) = v (get h0 a (ctr-1)) * v s); 
+	 gcut (fun _ -> v (get h2 res (ctr-1+0)) = v (get h0 a (ctr-1)) * v s); 
 	 cut (forall (i:nat). i < ctr ==> v (get h2 res i) = v (get h0 a i) * v s); 
-//	 cut (scalarProduct h0 h2 ctr a s res); 
-//	 cut (equal h0 a h2 a); 
-//	 cut (equalSub h0 res ctr h1 res ctr (length res - ctr));
+	 gcut (fun  _-> scalarProduct h0 h2 ctr a s res); 
+	 gcut (fun _ -> equal h0 a h2 a); 
+	 gcut (fun _ -> equalSub h0 res ctr h1 res ctr (length res - ctr));
 	 ()
 
 #reset-options
@@ -463,6 +463,7 @@ let aux_lemma_41 b =
 
 val aux_lemma_42: h:heap -> a:bigint{bound27 h a} -> z:uint63{v z < pow2 26} -> Lemma (forall (i:nat). i < norm_length ==> v (get h a i) * v z < pow2 53)
 let aux_lemma_42 h a z = 
+  admit(); // TODO
   cut (forall (i:nat). {:pattern (get h a i)} i < norm_length ==> (v (get h a i) < pow2 27)); 
   aux_lemma_41 z; 
   IntLibLemmas.pow2_exp 27 26;
@@ -708,7 +709,9 @@ let multiplication_step_p1 a b ctr c tmp =
   let h2 = ST.get() in 
   multiplication_step_lemma_02 h0 h1 h2 a b ctr c tmp;
   ()
-  
+
+#reset-options
+
 val helper_lemma_6: h0:heap -> h1:heap -> a:bigint -> b:bigint -> ctr:nat{ctr < norm_length} -> 
   c:bigint{disjoint a c /\ disjoint b c /\ length c >= 2 * norm_length - 1} -> 
   tmp:bigint{disjoint a tmp /\ disjoint b tmp /\ disjoint c tmp} -> Lemma 
@@ -717,6 +720,8 @@ val helper_lemma_6: h0:heap -> h1:heap -> a:bigint -> b:bigint -> ctr:nat{ctr < 
        /\ eval h0 c (2*norm_length-1) + pow2 (bitweight templ ctr) * eval h0 a (norm_length) * v (get h0 b ctr)  = eval h0 a (norm_length) * v (get h0 b ctr) * pow2 (bitweight templ ctr) + eval h0 c (2*norm_length-1) ))
 let helper_lemma_6 h0 h1 a b ctr c tmp = 
   ()
+
+#reset-options
 
 val multiplication_step: a:bigint -> b:bigint -> ctr:nat{ctr < norm_length} -> 
   c:bigint{disjoint a c /\ disjoint b c /\ length c >= 2*norm_length-1} -> 
@@ -819,6 +824,8 @@ assume val multiplication_aux_lemma: h0:heap -> h1:heap -> a:bigint -> b:bigint 
   (fun _ -> gmultiplication_aux_lemma h0 h1 a b ctr c tmp)
 *)
 
+#reset-options
+
 val multiplication_aux_lemma_2: h0:heap -> h1:heap -> h2:heap -> a:bigint -> b:bigint -> 
   ctr:nat{ctr <= norm_length} -> c:bigint{disjoint a c /\ disjoint b c /\ length c >= 2*norm_length-1} -> 
   tmp:bigint{disjoint a tmp /\ disjoint b tmp /\ disjoint c tmp} -> Lemma 
@@ -880,6 +887,8 @@ let ghelper_lemma_15 h0 h1 c =
   eq_lemma h0 h1 c empty;
   eval_null h1 c (2*norm_length - 1); 
   max_value_of_null_lemma h1 c (length c)
+
+#reset-options
 
 assume val helper_lemma_15: h0:heap -> h1:heap -> c:bigint{length c >= 2*norm_length-1} -> Lemma
     (requires (live h0 c /\ null h0 c /\ modifies_buf empty h0 h1))
@@ -960,7 +969,7 @@ val multiplication: c:bigint{length c >= 2*norm_length-1} -> a:bigint{disjoint c
        /\ maxValue h1 c (length c) <= norm_length * pow2 53 ))
 let multiplication c a b =
   let h0 = ST.get() in
-  let tmp = create #63 FStar.UInt63.zero norm_length in 
+  let tmp = create #63 SInt.UInt63.zero norm_length in 
   let h1 = ST.get() in
   multiplication_lemma_1 h0 h1 c a b; 
   multiplication_aux a b norm_length c tmp; 
@@ -981,6 +990,8 @@ let modulo_lemma a b = ()
 
 let satisfiesModuloConstraints (h:heap) (b:bigint) : GTot Type0 = 
   live h b /\ length b >= 2*norm_length-1 && maxValue h b (2*norm_length-1) * 6 < pow2 62
+
+#reset-options
 
 val times_5: x:uint63{5 * v x < pow2 63} -> Tot (y:uint63{v y = 5 * v x})
 let times_5 x = 
@@ -1104,6 +1115,8 @@ assume val freduce_degree_lemma:
     (fun _ -> gfreduce_degree_lemma h0 h1 b ctr)
 *)
 
+#reset-options
+
 val freduce_degree': 
   b:bigint -> ctr:nat{ctr < norm_length - 1} -> ST unit 
     (requires (fun h -> reducible h b ctr)) 
@@ -1111,7 +1124,6 @@ val freduce_degree':
       /\ eval h1 b (norm_length) % reveal prime = eval h0 b (norm_length+1+ctr) % reveal prime
       /\ modifies_buf (only b) h0 h1))
 let rec freduce_degree' b ctr' =
-  admit();
   let h0 = ST.get() in
   match ctr' with
   | 0 -> 
@@ -1121,9 +1133,9 @@ let rec freduce_degree' b ctr' =
     let bctr = bctr ^+ b5ctr in 
     upd b 0 bctr;
     let h1 = ST.get() in
-    freduce_degree_lemma h0 h1 b 0
-//    cut (True /\ eval h0 b (norm_length+1+0) % reveal prime = eval h1 b (norm_length+0) % reveal prime);
-//    cut (True /\ eval h0 b (norm_length+1) % reveal prime = eval h1 b (norm_length+0) % reveal prime)
+    freduce_degree_lemma h0 h1 b 0;
+    gcut (fun _ -> eval h0 b (norm_length+1+0) % reveal prime = eval h1 b (norm_length+0) % reveal prime);
+    gcut (fun _ -> eval h0 b (norm_length+1) % reveal prime = eval h1 b (norm_length+0) % reveal prime)
   | _ -> 
     let ctr = ctr' in
     let b5ctr = index b (ctr + norm_length) in 
@@ -1133,14 +1145,14 @@ let rec freduce_degree' b ctr' =
     upd b ctr bctr;
     let h1 = ST.get() in
     freduce_degree_lemma h0 h1 b ctr; 
-//    cut (True /\ eval h0 b (norm_length+1+ctr) % reveal prime = eval h1 b (norm_length+ctr) % reveal prime);
-//    cut(reducible h1 b (ctr-1)); 
+    gcut (fun _ -> eval h0 b (norm_length+1+ctr) % reveal prime = eval h1 b (norm_length+ctr) % reveal prime);
+    gcut(fun _ -> reducible h1 b (ctr-1)); 
     freduce_degree' b (ctr-1); 
     let h2 = ST.get() in 
     cut (forall (i:nat). {:pattern (v (get h1 b i))} (i > ctr /\ i < 2*norm_length-1) ==>
 	   v (get h1 b i) = v (get h0 b i)); 
-//    cut(untouched h0 h2 b ctr);
-//    cut (times5 h0 h2 b ctr) ;
+    gcut(fun _ -> untouched h0 h2 b ctr);
+    gcut (fun _ -> times5 h0 h2 b ctr) ;
     ()
 
 val aux_lemma_4': h:heap -> b:bigint -> Lemma
@@ -1192,6 +1204,8 @@ val helper_lemma_2: pb:nat -> pc:pos -> a0:nat -> b:nat ->
   Lemma  (ensures ((pb*pc) * a0/pc + (pb * (a0 % pc) + b) = pb * a0 + b))
 let helper_lemma_2 pb pc a0 b = ()
 
+#reset-options "--z3timeout 10"
+
 abstract val geval_carry_lemma: ha:heap -> a:bigint{live ha a /\ length a >= norm_length+1} -> 
   hb:heap -> b:bigint{live hb b /\ length b >= norm_length+1} -> ctr:nat{ctr < norm_length} -> GLemma unit
     (requires (v (get hb b ctr) = v (get ha a ctr) % pow2 (templ ctr)
@@ -1200,7 +1214,6 @@ abstract val geval_carry_lemma: ha:heap -> a:bigint{live ha a /\ length a >= nor
 	  (i < norm_length+1 /\ i <> ctr /\ i <> ctr+1) ==> v (get hb b i) = v (get ha a i)) ))
     (ensures (eval hb b (norm_length+1) = eval ha a (norm_length+1)))
 let geval_carry_lemma ha a hb b ctr =
-  admit();
   eval_eq_lemma ha hb a b ctr;
   cut(True /\ eval hb b (ctr+2) = pow2 (bitweight templ (ctr+1)) * v (get hb b (ctr+1)) + eval hb b (ctr+1)); 
   cut(True /\ eval hb b (ctr+2) = pow2 (bitweight templ (ctr+1)) * v (get hb b (ctr+1)) + (pow2 (bitweight templ ctr) * v (get hb b ctr) + eval hb b ctr));  
@@ -1219,7 +1232,7 @@ let geval_carry_lemma ha a hb b ctr =
   cut(True /\ eval hb b (ctr+2) = 
 	      pow2 (bitweight templ (ctr+1)) * v (get ha a (ctr+1)) 
 	      + (pow2 (bitweight templ ctr) * v (get ha a ctr) + eval hb b ctr));  
-//  cut(True /\ eval hb b (ctr+2) = eval ha a (ctr+2)); 
+  gcut(fun _ -> eval hb b (ctr+2) = eval ha a (ctr+2)); 
   eval_partial_eq_lemma ha hb a b (ctr+2) (norm_length+1)
 
 #reset-options
@@ -1288,9 +1301,9 @@ val mod2_26: a:uint63 -> Tot (b:uint63{v b = v a % pow2 26})
 let mod2_26 a = 
   let mask = shift_left one 26 in
   IntLibLemmas.pow2_increases 63 26; 
-  let mask = FStar.UInt63.sub mask one in
+  let mask = SInt.UInt63.sub mask one in
   let res = a ^& mask in
-  Sint.ulogand_lemma_4 #63 a 26 mask;
+  SInt.ulogand_lemma_4 #63 a 26 mask;
   res
 
 let carriable (h:heap) (b:bigint) (ctr:nat{ctr <= norm_length}) : GTot Type0 =
@@ -1314,6 +1327,8 @@ let untouched_2 (h0:heap) (h1:heap) (b:bigint) (ctr:nat) : GTot Type0 =
   /\ (forall (i:nat). {:pattern (get h1 b i)}
       ((i < ctr \/ i >= norm_length+1) /\ i < length b) ==> v (get h0 b i) = v (get h1 b i))
 
+#reset-options
+
 val carry: b:bigint -> ctr:nat{ctr <= norm_length} -> ST unit
     (requires (fun h -> carriable h b ctr /\ carried h b ctr))
     (ensures (fun h0 _ h1 -> carried h1 b norm_length /\ untouched_2 h0 h1 b ctr
@@ -1321,7 +1336,6 @@ val carry: b:bigint -> ctr:nat{ctr <= norm_length} -> ST unit
 //      /\ v (get h1 b (norm_length)) = IntLib.div (v (get h0 b (norm_length-1))) (pow2 26)
       /\ modifies_buf (only b) h0 h1 ))
 let rec carry b i =
-  admit();
   let h0 = ST.get() in
   match norm_length - i with
   | 0 -> ()
@@ -1332,10 +1346,10 @@ let rec carry b i =
     upd b i ri; 
     let h1 = ST.get() in
     let c = (bi ^>> 26) in
-//    cut (v bi < pow2 63 /\ v c = IntLib.div (v bi) (pow2 26)); 
+    gcut (fun _ -> v bi < pow2 63 /\ v c = IntLib.div (v bi) (pow2 26)); 
     IntLibLemmas.pow2_div 63 26;
     (* TODO *)
-//    admitP (True /\ v c < pow2 (63 - 26)); 
+    gassume (fun _ -> v c < pow2 (63 - 26)); 
     let bip1 = index b (i+1) in
 //    assert(v bip1 = v (get h1 b (i+1))); 
 //    assert(v bip1 < pow2 (63 - 1)); 
@@ -1434,7 +1448,6 @@ val carry2: b:bigint -> ST unit
     /\ eval h1 b (norm_length+1) % reveal prime = eval h0 b (norm_length+1) % reveal prime
     /\ modifies_buf (only b) h0 h1))
 let rec carry2 b = 
-  admit();
   let h0 = ST.get() in
   pow2_3_lemma ();
   IntLibLemmas.pow2_exp 3 37;
@@ -1444,19 +1457,19 @@ let rec carry2 b =
   IntLibLemmas.pow2_increases 62 41;
   carry_top_to_0 b;
   let h1 = ST.get() in
-  upd b norm_length FStar.UInt63.zero;
+  upd b norm_length SInt.UInt63.zero;
   let h2 = ST.get() in
   eval_eq_lemma h1 h2 b b norm_length;
-//  cut (True /\ eval h2 b (norm_length+1) = eval h1 b (norm_length)); 
+  gcut (fun _ ->  eval h2 b (norm_length+1) = eval h1 b (norm_length)); 
   let bi = index b 0 in 
   let ri = mod2_26 bi in
 //  assert(v ri < pow2 26); 
   upd b 0 ri; 
   let h3 = ST.get() in
   let c = (bi ^>> 26) in
-//  cut (True /\ v bi < pow2 41); 
+  gcut (fun _ -> v bi < pow2 41); 
   // In the spec of >>, TODO
-//  admitP(True /\ v c < pow2 15); 
+  gassume (fun _ -> v c < pow2 15); 
   let bip1 = index b 1 in 
   auxiliary_lemma_2 bip1 c; 
   IntLibLemmas.pow2_increases 63 27;
@@ -1466,7 +1479,7 @@ let rec carry2 b =
   upd b 1 z;
   let h4 = ST.get() in 
   eval_carry_lemma h2 b h4 b 0; 
-//  cut(carriable2 h4 b 1);
+  gcut(fun _ -> carriable2 h4 b 1);
   carry2_aux b 1
   
 
@@ -1476,46 +1489,45 @@ val last_carry: b:bigint -> ST unit
     /\ eval h1 b norm_length % reveal prime = eval h0 b (norm_length+1) % reveal prime
     /\ modifies_buf (only b) h0 h1))
 let last_carry b =
-  admit();
   let h0 = ST.get() in
   let b0 = index b 0 in
   let btop = index b norm_length in 
-//  cut (v b0 < pow2 26 /\ v btop < 2); 
+  gcut (fun _ -> v b0 < pow2 26 /\ v btop < 2); 
   pow2_3_lemma ();
-//  cut (5 * v btop < pow2 3 /\ True); 
+  gcut (fun _ -> 5 * v btop < pow2 3 /\ True); 
   IntLibLemmas.pow2_increases 26 3;
   IntLibLemmas.pow2_doubles 26;
   IntLibLemmas.pow2_increases 63 27;
-//  cut(v b0 + 5 * v btop < pow2 27 /\ True); 
+  gcut(fun _ -> v b0 + 5 * v btop < pow2 27 /\ True); 
   let btop_5 = times_5 btop in  
-//  upd b 0 (b0 ^+ btop_5); 
+  upd b 0 (b0 ^+ btop_5); 
   let h1 = ST.get() in
   freduce_degree_lemma h0 h1 b 0;
-//  upd b norm_length FStar.UInt63.zero;
+  upd b norm_length SInt.UInt63.zero;
   let h2 = ST.get() in
   eval_eq_lemma h1 h2 b b norm_length;
-//  cut (True /\ eval h2 b (norm_length+1) = eval h1 b norm_length);
+  gcut (fun _ -> eval h2 b (norm_length+1) = eval h1 b norm_length);
   let bi = index b 0 in 
   let ri = mod2_26 bi in
 //  assert(v ri < pow2 26); 
-//  upd b 0 ri; 
+  upd b 0 ri; 
   let h3 = ST.get() in
   let c = (bi ^>> 26) in
-//  cut (True /\ v bi < pow2 26 + 5); 
-//  cut (v bi >= pow2 26 ==> v (get h3 b 1) < pow2 15); 
+  gcut (fun _ -> v bi < pow2 26 + 5); 
+  gcut (fun _ -> v bi >= pow2 26 ==> v (get h3 b 1) < pow2 15); 
   // In the spec of >>, TODO
-//  admitP(v bi >= pow2 26 ==> v c = 1); 
+  gassume (fun _ -> v bi >= pow2 26 ==> v c = 1); 
   let bip1 = index b 1 in 
   auxiliary_lemma_2 bip1 c; 
   IntLibLemmas.pow2_increases 63 27;
   IntLibLemmas.pow2_doubles 26;
   IntLibLemmas.pow2_increases 26 15; 
   let z = bip1 ^+ c in 
-//  upd b 1 z;
+  upd b 1 z;
   let h4 = ST.get() in 
   eval_carry_lemma h2 b h4 b 0; 
-//  cut (True /\ v (get h4 b 1) < pow2 26); 
-//  cut (True /\ norm h4 b);
+  gcut (fun _ -> v (get h4 b 1) < pow2 26); 
+  gcut (fun _ -> norm h4 b);
   ()
 
 val modulo: b:bigint -> ST unit
@@ -1528,10 +1540,10 @@ let modulo b =
   let h0 = ST.get() in
   freduce_degree b; 
   let h1 = ST.get() in
-//  upd b norm_length FStar.UInt63.zero;
+  upd b norm_length SInt.UInt63.zero;
   let h2 = ST.get() in
   eval_eq_lemma h1 h2 b b norm_length;
-//  cut (True /\ eval h2 b (norm_length+1) = eval h1 b norm_length);
+  gcut (fun _ -> eval h2 b (norm_length+1) = eval h1 b norm_length);
   carry b 0; 
   let h3 = ST.get() in
   carry2 b; 
@@ -1546,7 +1558,7 @@ val freduce_coefficients: b:bigint -> ST unit
     /\ modifies_buf (only b) h0 h1))
 let freduce_coefficients b = 
   let h0 = ST.get() in
-  let tmp = create #63 FStar.UInt63.zero (2*norm_length-1) in
+  let tmp = create #63 SInt.UInt63.zero (2*norm_length-1) in
   let h1 = ST.get() in
   eq_lemma h0 h1 b empty; 
   eval_eq_lemma h0 h1 b b norm_length; 
