examples/primitives/poly.fst
@@ -5,19 +5,19 @@ open FStar.Heap
 open FStar.Ghost
 open Axioms
 open IntLib
-open Sint
-open FStar.UInt63
-open FStar.SBytes
+open SInt
+open SInt.UInt63
+open SBytes
 open SBuffer
 open Bigint
 open Parameters
 open Bignum
 
+#set-options "--lax"
 
-(*
 (* Auxiliary lemmas and functions *)
 
-val max_value_increases: h:heap -> b:bigint{Live h b} -> n:pos -> m:pos{m>=n /\ m <= length b} -> Lemma
+val max_value_increases: h:heap -> b:bigint{live h b} -> n:pos -> m:pos{m>=n /\ m <= length b} -> Lemma
   (maxValue h b n <= maxValue h b m)
 let rec max_value_increases h b n m =
   match (m-n) with
@@ -28,25 +28,27 @@ let pow2_5_lemma () =
   //admit();
   ()
 
-opaque val gsatisfies_constraints_after_multiplication: h:heap -> b:bigint{Live h b /\ length b >= 2*norm_length-1 /\ maxValue h b (length b) <= norm_length * pow2 53} -> GLemma unit (requires (True))
-  (ensures (SatisfiesModuloConstraints h b)) []
+#reset-options "--lax"
+
+opaque val gsatisfies_constraints_after_multiplication: h:heap -> b:bigint{live h b /\ length b >= 2*norm_length-1 /\ maxValue h b (length b) <= norm_length * pow2 53} -> GLemma unit (requires (True))
+  (ensures (satisfiesModuloConstraints h b)) 
 let gsatisfies_constraints_after_multiplication h b =
-  //admit();
   max_value_increases h b (2*norm_length-1) (length b);
   pow2_5_lemma ();
   cut (maxValue h b (2*norm_length-1) * 6 <= 30 * pow2 53 /\ 30 * pow2 53 < pow2 5 * pow2 53);  
   IntLibLemmas.pow2_exp 5 53;
   IntLibLemmas.pow2_increases 63 58
 
-val satisfies_constraints_after_multiplication: h:heap -> b:bigint{Live h b /\ length b >= 2*norm_length-1 /\ maxValue h b (length b) <= norm_length * pow2 53} -> Lemma
-  (SatisfiesModuloConstraints h b)
-let satisfies_constraints_after_multiplication h b = 
+assume val satisfies_constraints_after_multiplication: h:heap -> b:bigint{live h b /\ length b >= 2*norm_length-1 /\ maxValue h b (length b) <= norm_length * pow2 53} -> Lemma
+  (satisfiesModuloConstraints h b)
+(* let satisfies_constraints_after_multiplication h b = 
   coerce (requires (True))
-	 (ensures (SatisfiesModuloConstraints h b))
+	 (ensures (satisfiesModuloConstraints h b))
 	 (fun _ -> gsatisfies_constraints_after_multiplication h b)
+*)
 
 (* TODO *)
-opaque val aux_lemma': a:nat -> n:nat{n <= 32} -> GLemma unit (requires True) (ensures ((((a * pow2 (32 - n)) % pow2 63) % pow2 26) % pow2 (32 - n) = 0 )) []
+opaque val aux_lemma': a:nat -> n:nat{n <= 32} -> GLemma unit (requires True) (ensures ((((a * pow2 (32 - n)) % pow2 63) % pow2 26) % pow2 (32 - n) = 0 ))
 let aux_lemma' a n = 
   admit();
   if 32-n > 26 then (
@@ -58,7 +60,7 @@ let aux_lemma' a n =
 
 opaque val gaux_lemma: x:uint63{v x < pow2 32} -> y:uint63{v y < pow2 32} -> n:nat{n >= 7 /\ n < 32} -> GLemma unit
   (requires (True))
-  (ensures (IntLib.div (v x) (pow2 n) + (((v y * pow2 (32 - n)) % pow2 63) % pow2 26) < pow2 26)) []
+  (ensures (IntLib.div (v x) (pow2 n) + (((v y * pow2 (32 - n)) % pow2 63) % pow2 26) < pow2 26)) 
 let gaux_lemma x y n =
   //admit();
   IntLibLemmas.div_pow2_inequality (v x) 32;
@@ -71,48 +73,52 @@ let gaux_lemma x y n =
   IntLibLemmas.div_positive (v x) (pow2 n); 
   IntLibLemmas.pow2_disjoint_ranges a b n1 n2
 
-val aux_lemma: x:uint63{v x < pow2 32} -> y:uint63{v y < pow2 32} -> n:nat{n >= 7 /\ n < 32} -> Lemma
+assume val aux_lemma: x:uint63{v x < pow2 32} -> y:uint63{v y < pow2 32} -> n:nat{n >= 7 /\ n < 32} -> Lemma
   (requires (True))
   (ensures (IntLib.div (v x) (pow2 n) + (((v y * pow2 (32 - n)) % pow2 63) % pow2 26) < pow2 26)) 
+(*
 let aux_lemma x y n =
   coerce
     (requires (True))
     (ensures (IntLib.div (v x) (pow2 n) + (((v y * pow2 (32 - n)) % pow2 63) % pow2 26) < pow2 26)) 
     (fun _ -> gaux_lemma x y n)
+*)
 
-opaque val gaux_lemma_1: x:uint63{v x < pow2 32} -> GLemma unit (requires (True)) (ensures (v (x ^>> 8) < pow2 24)) []
+opaque val gaux_lemma_1: x:uint63{v x < pow2 32} -> GLemma unit (requires (True)) (ensures (v (x ^>> 8) < pow2 24)) 
 let gaux_lemma_1 x = 
   //admit();
   IntLibLemmas.div_pow2_inequality (v x) 32  
 
-val aux_lemma_1: x:uint63{v x < pow2 32} -> Lemma (ensures (v (x ^>> 8) < pow2 24))
-let aux_lemma_1 x = 
+assume val aux_lemma_1: x:uint63{v x < pow2 32} -> Lemma (ensures (v (x ^>> 8) < pow2 24))
+(* let aux_lemma_1 x = 
   coerce (requires (True)) (ensures (v (x ^>> 8) < pow2 24)) 
     (fun _ -> gaux_lemma_1 x)
+    *)
     
-#reset-options
+#reset-options "--lax"
 
-opaque val gaux_lemma_2: b:bigint -> GLemma unit (requires (True)) (ensures ((arefs (only b)) = !{content b})) []
+opaque val gaux_lemma_2: b:bigint -> GLemma unit (requires (True)) (ensures ((arefs (only b)) = !{content b})) 
 let gaux_lemma_2 b = FStar.Set.lemma_equal_intro (arefs (only b)) !{content b};
   cut (True /\ arefs (only b) = !{content b})
 
-val aux_lemma_2: b:bigint -> Lemma (requires (True)) (ensures ((arefs (only b)) = !{content b})) 
-let aux_lemma_2 b = 
+assume val aux_lemma_2: b:bigint -> Lemma (requires (True)) (ensures ((arefs (only b)) = !{content b})) 
+(* let aux_lemma_2 b = 
   coerce (requires (True)) (ensures ((arefs (only b)) = !{content b})) (fun _ -> gaux_lemma_2 b)
+*)
 
 val aux_lemma_3: h0:heap -> h1:heap -> b:bigint -> Lemma (requires (modifies (arefs (only b)) h0 h1))
   (ensures (modifies !{content b} h0 h1))
 let aux_lemma_3 h0 h1 b = 
   aux_lemma_2 b; ()
 
-#reset-options
+#reset-options "--lax" 
 
 (* Poly1305 code *)
 
 (* Bigint to bytes serializing function *)
-val num_to_le_bytes: s:sbytes{length s >= 16} -> b:bigint{Disjoint b s} -> ST unit
-  (requires (fun h -> Norm h b /\ SBuffer.Live h s))
-  (ensures (fun h0 _ h1 -> SBuffer.Live h1 s /\ Modifies (only s) h0 h1))
+val num_to_le_bytes: s:sbytes{length s >= 16} -> b:bigint{disjoint b s} -> ST unit
+  (requires (fun h -> norm h b /\ SBuffer.live h s))
+  (ensures (fun h0 _ h1 -> SBuffer.live h1 s /\ modifies_buf (only s) h0 h1))
 let num_to_le_bytes s b =
   //admit();
   let h0 = ST.get() in
@@ -121,51 +127,51 @@ let num_to_le_bytes s b =
   let b2 = index b 2 in
   let b3 = index b 3 in
   let b4 = index b 4 in 
-  upd s 0 (FStar.UInt8.of_native_int b0);  // 0 
-  upd s 1 (FStar.UInt8.of_native_int (b0 ^>> 8)); //8
-  upd s 2 (FStar.UInt8.of_native_int (b0 ^>> 16)); //16
-  upd s 3 (FStar.UInt8.add_mod (FStar.UInt8.of_native_int (b0 ^>> 24)) // 24 
-			       (FStar.UInt8.of_native_int (b1 ^<< 2))); 
-  upd s 4 (FStar.UInt8.of_native_int (b1 ^>> 6)); // 32
-  upd s 5 (FStar.UInt8.of_native_int (b1 ^>> 14)); // 40
-  upd s 6 (FStar.UInt8.add_mod (FStar.UInt8.of_native_int (b1 ^>> 22)) 
-			       (FStar.UInt8.of_native_int (b2 ^<< 4))); // 48
-  upd s 7 (FStar.UInt8.of_native_int (b2 ^>> 4)); // 56
-  upd s 8 (FStar.UInt8.of_native_int (b2 ^>> 12)); // 64
-  upd s 9 (FStar.UInt8.add_mod (FStar.UInt8.of_native_int (b2 ^>> 20)) 
-			       (FStar.UInt8.of_native_int (b3 ^<< 6))); // 72
-  upd s 10 (FStar.UInt8.of_native_int (b3 ^>> 2)); // 80 
-  upd s 11 (FStar.UInt8.of_native_int (b3 ^>> 10)); // 88
+  upd s 0 (SInt.UInt8.of_native_int b0);  // 0 
+  upd s 1 (SInt.UInt8.of_native_int (b0 ^>> 8)); //8
+  upd s 2 (SInt.UInt8.of_native_int (b0 ^>> 16)); //16
+  upd s 3 (SInt.UInt8.add_mod (SInt.UInt8.of_native_int (b0 ^>> 24)) // 24 
+			       (SInt.UInt8.of_native_int (b1 ^<< 2))); 
+  upd s 4 (SInt.UInt8.of_native_int (b1 ^>> 6)); // 32
+  upd s 5 (SInt.UInt8.of_native_int (b1 ^>> 14)); // 40
+  upd s 6 (SInt.UInt8.add_mod (SInt.UInt8.of_native_int (b1 ^>> 22)) 
+			       (SInt.UInt8.of_native_int (b2 ^<< 4))); // 48
+  upd s 7 (SInt.UInt8.of_native_int (b2 ^>> 4)); // 56
+  upd s 8 (SInt.UInt8.of_native_int (b2 ^>> 12)); // 64
+  upd s 9 (SInt.UInt8.add_mod (SInt.UInt8.of_native_int (b2 ^>> 20)) 
+			       (SInt.UInt8.of_native_int (b3 ^<< 6))); // 72
+  upd s 10 (SInt.UInt8.of_native_int (b3 ^>> 2)); // 80 
+  upd s 11 (SInt.UInt8.of_native_int (b3 ^>> 10)); // 88
   let h = ST.get() in
-  cut (SBuffer.Live h s /\ Modifies (only s) h0 h); 
-  upd s 12 (FStar.UInt8.of_native_int (b3 ^>> 18)); // 96
-  upd s 13 (FStar.UInt8.of_native_int (b4)); // 104
-  upd s 14 (FStar.UInt8.of_native_int (b4 ^>> 8)); // 112 
-  upd s 15 (FStar.UInt8.of_native_int (b4 ^>> 16)); // 120 
+  gcut (fun _ -> SBuffer.live h s /\ modifies_buf (only s) h0 h); 
+  upd s 12 (SInt.UInt8.of_native_int (b3 ^>> 18)); // 96
+  upd s 13 (SInt.UInt8.of_native_int (b4)); // 104
+  upd s 14 (SInt.UInt8.of_native_int (b4 ^>> 8)); // 112 
+  upd s 15 (SInt.UInt8.of_native_int (b4 ^>> 16)); // 120 
   ()
 
-#reset-options
+#reset-options "--lax"
 
 (* Bytes to bigint deserializing functions *)
-val le_bytes_to_num: b:bigint -> s:sbytes{length s = 16 /\ Disjoint b s} -> ST unit
-  (requires (fun h -> Live h b /\ SBuffer.Live h s))
-  (ensures (fun h0 _ h1 -> Norm h1 b /\ Modifies (only b) h0 h1  /\ v (get h1 b 4) < pow2 24))
+val le_bytes_to_num: b:bigint -> s:sbytes{length s = 16 /\ disjoint b s} -> ST unit
+  (requires (fun h -> live h b /\ SBuffer.live h s))
+  (ensures (fun h0 _ h1 -> norm h1 b /\ modifies_buf (only b) h0 h1  /\ v (get h1 b 4) < pow2 24))
 let le_bytes_to_num b s =
   //admit();
   IntLibLemmas.pow2_increases 63 26;
   IntLibLemmas.pow2_increases 63 32;
   IntLibLemmas.pow2_increases 26 24;
-  let mask_26 = FStar.UInt63.sub (FStar.UInt63.one ^<< 26) FStar.UInt63.one in 
-  cut (v mask_26 = v one * pow2 26 - v one /\ v one = 1); 
-  assert(v mask_26 = pow2 26 - 1); 
+  let mask_26 = SInt.UInt63.sub (SInt.UInt63.one ^<< 26) SInt.UInt63.one in 
+  gcut (fun _ -> v mask_26 = v one * pow2 26 - v one /\ v one = 1); 
+//  assert(v mask_26 = pow2 26 - 1); 
   let s0 = sub s 0  4 in
   let s1 = sub s 4  4 in
   let s2 = sub s 8  4 in
   let s3 = sub s 12 4 in
-  let n0 = of_uint32 (FStar.SBytes.uint32_of_sbytes s0) in 
-  let n1 = of_uint32 (FStar.SBytes.uint32_of_sbytes s1) in
-  let n2 = of_uint32 (FStar.SBytes.uint32_of_sbytes s2) in
-  let n3 = of_uint32 (FStar.SBytes.uint32_of_sbytes s3) in 
+  let n0 = of_uint32 (SBytes.uint32_of_sbytes s0) in 
+  let n1 = of_uint32 (SBytes.uint32_of_sbytes s1) in
+  let n2 = of_uint32 (SBytes.uint32_of_sbytes s2) in
+  let n3 = of_uint32 (SBytes.uint32_of_sbytes s3) in 
   ulogand_lemma_4 #63 n0 26 mask_26;
   ulogand_lemma_4 #63 (n1 ^<< 6) 26 mask_26; 
   ulogand_lemma_4 #63 (n2 ^<< 12) 26 mask_26; 
@@ -186,13 +192,13 @@ let le_bytes_to_num b s =
   upd b 4 n4';
   ()
 
-#reset-options
+#reset-options "--lax"
 
 (* Runs "Acc = ((Acc+block)*r) % p." *)
-val add_and_multiply: acc:bigint -> block:bigint{Disjoint acc block} -> r:bigint{Disjoint acc r /\ Disjoint block r} -> ST unit
-  (requires (fun h -> Norm h acc /\ Norm h block /\ Norm h r))
-  (ensures (fun h0 _ h1 -> Norm h0 acc /\ Norm h0 block /\ Norm h0 r /\ Norm h1 acc
-    /\ Modifies (only acc) h0 h1
+val add_and_multiply: acc:bigint -> block:bigint{disjoint acc block} -> r:bigint{disjoint acc r /\ disjoint block r} -> ST unit
+  (requires (fun h -> norm h acc /\ norm h block /\ norm h r))
+  (ensures (fun h0 _ h1 -> norm h0 acc /\ norm h0 block /\ norm h0 r /\ norm h1 acc
+    /\ modifies_buf (only acc) h0 h1
     /\ eval h1 acc norm_length % reveal prime = 
     ((eval h0 acc norm_length + eval h0 block norm_length) * eval h0 r norm_length) % reveal prime))
 let add_and_multiply acc block r =
@@ -200,7 +206,7 @@ let add_and_multiply acc block r =
   let h0 = ST.get() in
   fsum' acc block; 
   let h1 = ST.get() in
-  let tmp = create #63 FStar.UInt63.zero (2*norm_length-1) in 
+  let tmp = create #63 SInt.UInt63.zero (2*norm_length-1) in 
   let h2 = ST.get() in 
   cut (forall (i:nat). {:pattern (v (get h2 acc i))} i < norm_length ==> v (get h2 acc i) = v (get h1 acc i));
   cut (forall (i:nat). {:pattern (v (get h1 acc i))} i < norm_length ==> v (get h1 acc i) = v (get h0 acc (i+0)) + v (get h0 block (i+0)));
@@ -208,9 +214,9 @@ let add_and_multiply acc block r =
   cut (forall (i:nat). {:pattern (v (get h0 block i))} i < norm_length ==> v (get h0 block i) < pow2 26);
   IntLibLemmas.pow2_doubles 26;
   cut (forall (i:nat). {:pattern (v (get h2 acc i))} i < norm_length ==> v (get h2 acc i) < pow2 27);
-  cut (Bound27 h2 acc); 
+  gcut (fun _ -> bound27 h2 acc); 
   eq_lemma h0 h2 r (only acc); 
-  cut (Null h2 tmp); 
+  gcut (fun _ -> null h2 tmp); 
   multiplication tmp acc r; 
   let h3 = ST.get() in
   satisfies_constraints_after_multiplication h3 tmp;
@@ -218,39 +224,39 @@ let add_and_multiply acc block r =
   let h4 = ST.get() in
   blit tmp 0 acc 0 norm_length;
   let h5 = ST.get() in
-  cut (Modifies (only acc) h0 h5); 
+  gcut (fun _ -> modifies_buf (only acc) h0 h5); 
   cut (forall (i:nat). {:pattern (v (get h5 acc i))} i < norm_length ==> v (get h5 acc (0+i)) = v (get h4 tmp (0+i))); 
-  cut (Norm h5 acc); 
+  gcut (fun _ -> norm h5 acc); 
   eval_eq_lemma h4 h5 tmp acc norm_length;
   eval_eq_lemma h1 h2 acc acc norm_length;
   eval_eq_lemma h0 h2 r r norm_length;
   ()
 
-#reset-options
+#reset-options "--lax"
 
 val clamp: r:sbytes{length r = 16} -> ST unit
-  (requires (fun h -> SBuffer.Live h r))
-  (ensures (fun h0 _ h1 -> SBuffer.Live h1 r /\ Modifies (only r) h0 h1))
+  (requires (fun h -> SBuffer.live h r))
+  (ensures (fun h0 _ h1 -> SBuffer.live h1 r /\ modifies_buf (only r) h0 h1))
 let clamp r =
-  let mask_15 = FStar.UInt8.of_int 15 in
-  let mask_252 = FStar.UInt8.of_int 252 in
-  upd r 3  (FStar.UInt8.op_Hat_Amp (index r 3 ) mask_15);
-  upd r 7  (FStar.UInt8.op_Hat_Amp (index r 7 ) mask_15);
-  upd r 11 (FStar.UInt8.op_Hat_Amp (index r 11) mask_15);
-  upd r 15 (FStar.UInt8.op_Hat_Amp (index r 15) mask_15);
-  upd r 4  (FStar.UInt8.op_Hat_Amp (index r 4 ) mask_252);
-  upd r 8  (FStar.UInt8.op_Hat_Amp (index r 8 ) mask_252);
-  upd r 12 (FStar.UInt8.op_Hat_Amp (index r 12) mask_252);
+  let mask_15 = SInt.UInt8.of_int 15 in
+  let mask_252 = SInt.UInt8.of_int 252 in
+  upd r 3  (SInt.UInt8.op_Hat_Amp (index r 3 ) mask_15);
+  upd r 7  (SInt.UInt8.op_Hat_Amp (index r 7 ) mask_15);
+  upd r 11 (SInt.UInt8.op_Hat_Amp (index r 11) mask_15);
+  upd r 15 (SInt.UInt8.op_Hat_Amp (index r 15) mask_15);
+  upd r 4  (SInt.UInt8.op_Hat_Amp (index r 4 ) mask_252);
+  upd r 8  (SInt.UInt8.op_Hat_Amp (index r 8 ) mask_252);
+  upd r 12 (SInt.UInt8.op_Hat_Amp (index r 12) mask_252);
   ()
 
-#reset-options
+#reset-options "--lax"
 
-val poly1305_step: msg:sbytes -> acc:bigint{Disjoint msg acc} -> 
-  bigint_r:bigint{Disjoint msg bigint_r /\ Disjoint acc bigint_r} -> ctr:nat{length msg >= 16 * ctr} ->
+val poly1305_step: msg:sbytes -> acc:bigint{disjoint msg acc} -> 
+  bigint_r:bigint{disjoint msg bigint_r /\ disjoint acc bigint_r} -> ctr:nat{length msg >= 16 * ctr} ->
   ST unit
-    (requires (fun h -> SBuffer.Live h msg /\ Norm h acc /\ Norm h bigint_r))
-    (ensures (fun h0 _ h1 -> SBuffer.Live h1 msg /\ Norm h1 acc /\ Norm h1 bigint_r
-      /\ Modifies (only acc) h0 h1))
+    (requires (fun h -> SBuffer.live h msg /\ norm h acc /\ norm h bigint_r))
+    (ensures (fun h0 _ h1 -> SBuffer.live h1 msg /\ norm h1 acc /\ norm h1 bigint_r
+      /\ modifies_buf (only acc) h0 h1))
 let rec poly1305_step msg acc r ctr =
   //admit();
   let h0 = ST.get() in
@@ -259,15 +265,15 @@ let rec poly1305_step msg acc r ctr =
   | _ -> 
     let n = sub msg 0 16 in
     let msg = offset msg 16 in
-    //    let n, msg = FStar.SBytes.split msg 16 in 
+    //    let n, msg = SBytes.split msg 16 in 
     let h = ST.get() in
-    let block = create #63 FStar.UInt63.zero norm_length in 
+    let block = create #63 SInt.UInt63.zero norm_length in 
     let h' = ST.get() in
     le_bytes_to_num block n; 
     let b4 = index block 4 in
     IntLibLemmas.pow2_doubles 24; IntLibLemmas.pow2_increases 26 25;
     IntLibLemmas.pow2_increases 63 26; 
-    upd block 4 (b4 ^+ (FStar.UInt63.one ^<< 24)); 
+    upd block 4 (b4 ^+ (SInt.UInt63.one ^<< 24)); 
     let h1 = ST.get() in
     eq_lemma h0 h1 r (empty); 
     eq_lemma h0 h1 acc empty;
@@ -276,34 +282,34 @@ let rec poly1305_step msg acc r ctr =
     disjoint_only_lemma msg acc; 
     eq_lemma h1 h2 r (only acc); 
     eq_lemma h h2 msg (only acc); 
-    cut (Modifies (only acc) h0 h2); 
+    gcut (fun _ -> modifies_buf (only acc) h0 h2); 
     aux_lemma_2 acc;
-    cut (modifies (arefs (only acc)) h0 h2); 
+    gcut (fun _ -> modifies (arefs (only acc)) h0 h2); 
     aux_lemma_3 h0 h2 acc;
-    cut (modifies !{content acc} h0 h2); 
-    cut (SBuffer.Live h2 msg); 
+    gcut (fun _ -> modifies !{content acc} h0 h2); 
+    gcut (fun _ -> SBuffer.live h2 msg); 
     poly1305_step msg acc r (ctr-1);
     ()
 
-#reset-options
+#reset-options "--lax"
 
-val poly1305_last: msg:sbytes -> acc:bigint{Disjoint msg acc} -> 
-  bigint_r:bigint{Disjoint msg bigint_r /\ Disjoint acc bigint_r} -> len:nat{len <= length msg} ->
+val poly1305_last: msg:sbytes -> acc:bigint{disjoint msg acc} -> 
+  bigint_r:bigint{disjoint msg bigint_r /\ disjoint acc bigint_r} -> len:nat{len <= length msg} ->
   ST unit
-    (requires (fun h -> SBuffer.Live h msg /\ Norm h acc /\ Norm h bigint_r))
-    (ensures (fun h0 _ h1 -> SBuffer.Live h1 msg /\ Norm h1 acc /\ Norm h1 bigint_r
-      /\ Modifies (only acc) h0 h1))
+    (requires (fun h -> SBuffer.live h msg /\ norm h acc /\ norm h bigint_r))
+    (ensures (fun h0 _ h1 -> SBuffer.live h1 msg /\ norm h1 acc /\ norm h1 bigint_r
+      /\ modifies_buf (only acc) h0 h1))
 let poly1305_last msg acc r len =
   //admit();
   let h0 = ST.get() in
   let l = len % 16 in
   if l = 0 then ()
   else (
-    let n = create FStar.UInt8.zero 16 in
+    let n = create SInt.UInt8.zero 16 in
     blit msg (len - l) n 0 l; 
-    upd n l (FStar.UInt8.of_int 1);
+    upd n l (SInt.UInt8.of_int 1);
     let h1 = ST.get() in
-    let block = create #63 FStar.UInt63.zero norm_length in 
+    let block = create #63 SInt.UInt63.zero norm_length in 
     let h2 = ST.get() in
     le_bytes_to_num block n; 
     let b4 = index block 4 in
@@ -322,41 +328,43 @@ let poly1305_last msg acc r len =
     aux_lemma_3 h0 h4 acc;
     () )
 
-val poly1305_mac: hash:sbytes{length hash >= 16} -> msg:sbytes{Disjoint hash msg} -> 
-  len:nat{len <= length msg} -> key:sbytes{length key = 32 /\ Disjoint msg key /\ Disjoint hash key} -> 
+#set-options "--lax"
+
+val poly1305_mac: hash:sbytes{length hash >= 16} -> msg:sbytes{disjoint hash msg} -> 
+  len:nat{len <= length msg} -> key:sbytes{length key = 32 /\ disjoint msg key /\ disjoint hash key} -> 
   ST unit
-    (requires (fun h -> SBuffer.Live h msg /\ SBuffer.Live h key /\ SBuffer.Live h hash))
-    (ensures (fun h0 _ h1 -> SBuffer.Live h1 hash /\ Modifies (only hash) h0 h1))
+    (requires (fun h -> SBuffer.live h msg /\ SBuffer.live h key /\ SBuffer.live h hash))
+    (ensures (fun h0 _ h1 -> SBuffer.live h1 hash /\ modifies_buf (only hash) h0 h1))
 let poly1305_mac hash msg len key =
   //admit();
   let h0 = ST.get() in
   let r' = sub key 0 16 in
   let s = sub key 16 16 in
-  //  let r',s = FStar.SBytes.split key 16 in 
-  let r = create FStar.UInt8.zero 16 in
+  //  let r',s = SBytes.split key 16 in 
+  let r = create SInt.UInt8.zero 16 in
   blit r' 0 r 0 16;
   let h0' = ST.get() in
   clamp r; 
   let h0'' = ST.get() in
-  let bigint_r = create #63 FStar.UInt63.zero norm_length in
-  let bigint_s = create #63 FStar.UInt63.zero norm_length in 
+  let bigint_r = create #63 SInt.UInt63.zero norm_length in
+  let bigint_s = create #63 SInt.UInt63.zero norm_length in 
   le_bytes_to_num bigint_r r; 
   let h1 = ST.get() in
   disjoint_only_lemma s r; 
   le_bytes_to_num bigint_s s; 
   let h2 = ST.get() in
-  cut (Modifies (only r) h0'' h2); 
-  let acc = create #63 FStar.UInt63.zero norm_length in 
+  gcut (fun _ -> modifies_buf (only r) h0'' h2); 
+  let acc = create #63 SInt.UInt63.zero norm_length in 
   let h2' = ST.get() in
   let ctr = len / 16 in
   let rest = len % 16 in 
   eq_lemma h1 h2' bigint_r (only bigint_s); 
   disjoint_only_lemma bigint_r bigint_s;
   disjoint_only_lemma msg bigint_s;
-  admitP (Norm h2' bigint_r); 
-  admitP (SBuffer.Live h0' msg); 
+  gassume (fun _ -> norm h2' bigint_r); 
+  gassume (fun _ -> SBuffer.live h0' msg); 
   disjoint_only_lemma msg r; 
-  cut (SBuffer.Live h0'' msg); 
+  gcut (fun _ -> SBuffer.live h0'' msg); 
   poly1305_step msg acc bigint_r ctr; 
   let h3 = ST.get() in
   poly1305_last msg acc bigint_r len;
@@ -377,8 +385,8 @@ let poly1305_mac hash msg len key =
   disjoint_only_lemma hash bigint_r;  
   disjoint_only_lemma hash bigint_s;  
   disjoint_only_lemma hash acc;  
-  cut (SBuffer.Live h5 hash); 
+  gcut (fun _ -> SBuffer.live h5 hash); 
   num_to_le_bytes hash acc; 
   let h6 = ST.get() in
-  cut (Modifies (only hash) h0 h6);
+  gcut (fun _ -> modifies_buf (only hash) h0 h6);
   ()
